verif/btrees/verif_putrecord.v
@@ -15,6 +15,7 @@ Require Import verif_newnode.
 Require Import verif_movetokey.
 Require Import verif_currnode.
 Require Import verif_entryindex.*)
+
 Require Import verif_splitnode_part0. (*for Lemma upd_Znth_twice*)
 
 (* integrity of a new root *)
@@ -78,16 +79,25 @@ Proof. induction l; simpl; intros. contradiction.
   + destruct (Ptrofs.eq (entry_key a) k). inv H. auto.
 Qed.
 
-Lemma LeafEntry_entry_numrec_one {X e} (E: @LeafEntry X e): entry_numrec e =1.
-Proof. destruct e; [ trivial | simpl in E; contradiction]. Qed.
+Lemma Znth_option_key_in_le_true {X e}: forall l i, Znth_option i l = Some e ->
+      @key_in_le X (entry_key e) l = true.
+Proof.
+  induction l; simpl; intros.
+  rewrite Znth_option_nil in H; discriminate. 
+  destruct (zeq 0 i). 
+  + subst. rewrite Znth_option_0 in H; trivial. inv H; simpl. rewrite Ptrofs.eq_true; trivial.
+  + rewrite Znth_option_cons in H; trivial. apply IHl in H. rewrite H.
+    destruct (Ptrofs.eq (entry_key a) (entry_key e)); trivial.
+Qed.
+
 
 Lemma body_putEntry: semax_body Vprog Gprog f_putEntry putEntry_spec.
 Proof.
-  start_function.
+  start_function. rename H7 into ENotVundef.
   rename H0 into Hleaf. assert (EN:= LeafEntry_entry_numrec_one Hleaf).
   rename H1 into H0; rename H2 into H1; rename H3 into H2; rename H4 into H3;
   rename H5 into H4; rename H6 into H5;
-  rename H7 into EMPENTRY.
+  rename H8 into EMPENTRY.
   unfold cursor_rep. Intros anc_end. Intros idx_end.
   destruct r as [root prel]. pose (r:=(root,prel)).
   forward.                      (* t'44=cursor->level *)
@@ -119,7 +129,7 @@ Proof.
                                  temp _key (Vptrofs oldk)) 
                      SEP (cursor_rep [] r pc; mem_mgr gv; 
                             btnode_rep (empty_node false true true vnewnode); 
-                            relation_rep (root, prel); (* entry_rep e; *) data_at Tsh tentry (entry_val_rep e) pe)).
+                            relation_rep (root, prel); (* entry_rep e; *) data_at (*Tsh*)sh tentry (entry_val_rep e) pe)).
 (*    + apply denote_tc_test_eq_split.
       replace (vnewnode) with (getval (empty_node false true true vnewnode)). entailer!.
       simpl. auto.
@@ -273,13 +283,15 @@ Proof.
       forward.                  (* t'41=t'13->numKeys *)
       sep_apply (fold_btnode_rep ptr0). fold currnode.
       clear ent_end. deadvars!.
-      assert (H99: 0 <= entryidx < Zlength le). {
+      assert (H99: 0 <= entryidx < Zlength le /\ partial_cursor_correct c' (btnode val ptr0 le isLeaf First Last x) root ). {
           destruct H. red in H; simpl in H.
           destruct (Znth_option entryidx le) eqn:?H; try contradiction.
           destruct e0; try contradiction.
-          apply Znth_option_some in H9. auto. }
+          apply Znth_option_some in H9. split. auto. apply H. }
+      destruct H99 as [H99 PCC].
       assert (H98: Zlength le <= Fanout). {apply H2 in SUBNODE.
           apply node_wf_numKeys in SUBNODE. simpl in SUBNODE. rep_lia. }
+
      forward_if(PROP ( )
      LOCAL (temp _t'56 (Vint (Int.repr (Zlength (node_le currnode))));
      temp _t'15 (Vint (Int.repr entryidx)); 
@@ -291,7 +303,7 @@ Proof.
        (Vptrofs (Ptrofs.repr (get_numrec (root, prel)(* + entry_numrec e - 1*))),
        Vint (Int.repr (get_depth r)))) prel; btnode_rep currnode -* btnode_rep root;
      cursor_rep ((currnode, entryidx) :: c') r pc; (*entry_rep e;*)
-     data_at Ews tentry (entry_val_rep e) pe; mem_mgr gv)).
+     data_at sh tentry (entry_val_rep e) pe; mem_mgr gv)).
       {
         sep_apply modus_ponens_wand.
         forward_call(r,c,pc (* ,(get_numrec (root, prel) + entry_numrec e - 1) *) ). (* t'15=currnode(cursor) *)
@@ -330,12 +342,34 @@ Proof.
           (* destruct en; inversion HeqENVRe; subst vn sn; clear HeqENVRe; simpl in *.*
              Maybe it's enough to just remember that vn is a Vptrofs, rather than dsicriminating on sn, like this:*)
           assert (XX: exists kn, vn = Vptrofs kn /\ kn = entry_key en). { destruct en; simpl in HeqENVRe; inv HeqENVRe; eexists; split; reflexivity. }
-          destruct XX as [kn [? KN]]; subst vn kn.
+          destruct XX as [kn [? KN]]; subst vn kn; simpl.
+          unfold sem_cast_i2bool, Int64.eq. simpl. rewrite 2 int64_unsigned_ptrofs_toint by trivial. (*64bit*)
+          specialize (Ptrofs.eq_spec (entry_key en) k). 
+          specialize (Znth_option_key_in_le_true _ _ Hen); intros HH.
+          destruct (Ptrofs.eq (entry_key en) k); intros X.
+          * subst k. rewrite HH in HeqKeyInLe. subst KeyInLe. rewrite zeq_true; trivial.
+         (* * destruct (zeq (Ptrofs.unsigned (entry_key en)) (Ptrofs.unsigned k)).
+            - assert (Ptrofs.repr (Ptrofs.unsigned (entry_key en)) = Ptrofs.repr (Ptrofs.unsigned k)). rewrite e; trivial.
+               rewrite 2 Ptrofs.repr_unsigned in H6. elim X; trivial. 
+            - (*simpl. destruct KeyInLe; trivial.xx
+              destruct (key_in_le_true _ _ HeqKeyInLe) as [HT [entryE [TL [EE1 [EE2 EE3]]]]]; clear HeqKeyInLe.
+              apply Ptrofs.same_if_eq in EE2. subst k le. apply in_app_or in EnLe. destruct EnLe.
+              ++ apply Ptrofs.same_if_eq. specialize (EE3 _ H6).  admit.
+              ++  apply EE3 in H6.  specialize (key_in_le_false _ _ HeqKeyInLe _ EnLe); intros X; simpl in X.
+             simpl. unfold Ptrofs.eq in X. rewrite Int64.eq_false; simpl; trivial.
+             unfold Ptrofs.to_int64. if_tac in X. discriminate. intros N. clear - N H6.
+             rewrite <- ! int64_unsigned_ptrofs_toint in N; trivial.
+             rewrite <- ! int64_unsigned_ptrofs_toint in H6; trivial.
+             rewrite ! Int64.repr_unsigned in N. rewrite N in H6. apply H6; trivial.*)
+         (* lia.  
+(*           Search key_in_le.
+          destruct (zeq (Ptrofs.unsigned (entry_key en)) (Ptrofs.unsigned k)).*)
           destruct KeyInLe.
             * destruct (key_in_le_true _ _ HeqKeyInLe) as [HT [entryE [TL [EE1 [EE2 EE3]]]]]; clear HeqKeyInLe.
               (*Here is where we need to know in he leaf case that the cursor points to where the key should be if already,
-               to deduce that k0=k 
-              unfold entry_key in EE2. destruct e; simpl in H10. 2: simpl in Hleaf; contradiction.
+               to deduce that k0=k *)
+              destruct (). if_tac.
+              unfold entry_key in EE2.  destruct entryE; simpl. 2:{ simpl in *. contradiction. simpl in Hleaf; contradiction.
               simpl in *. Print entry_depth.
               -- destruct entryE; simpl in H11; simpl.
                  ++ apply Ptrofs.same_if_eq in EE2; subst k0.
@@ -357,15 +391,17 @@ Proof.
 
                 remember (Znth entryidx (map entry_val_rep le)) as e3. destruct e3; simpl in *.
                 destruct v; try contradiction.
-                destruct v0; try contradiction. clear - Heqee.  Print entry_val_rep. Print entry_key.*) admit.
-           * specialize (key_in_le_false _ _ HeqKeyInLe _ EnLe); intros X; simpl in X.
-             simpl. unfold Ptrofs.eq in X. rewrite Int64.eq_false; simpl; trivial.
-             unfold Ptrofs.to_int64. if_tac in X. discriminate. intros N. clear - N H6.
-             rewrite <- ! int64_unsigned_ptrofs_toint in N; trivial.
-             rewrite <- ! int64_unsigned_ptrofs_toint in H6; trivial.
-             rewrite ! Int64.repr_unsigned in N. rewrite N in H6. apply H6; trivial.
+                destruct v0; try contradiction. clear - Heqee.  Print entry_val_rep. Print entry_key.*)
+                admit. *)
+           * destruct KeyInLe. 
+             ++ destruct (key_in_le_true _ _ HeqKeyInLe) as [FRONT [E [TAIL [EE1 [EE2 EE3]]]]].
+                destruct (zeq (Ptrofs.unsigned (entry_key en)) (Ptrofs.unsigned k)); simpl; trivial.
+                admit.
+             ++ specialize (key_in_le_false _ _ HeqKeyInLe _ EnLe); intros Y; simpl in Y.
+                unfold Ptrofs.eq in Y. destruct (zeq (Ptrofs.unsigned (entry_key en)) (Ptrofs.unsigned k)). inv Y. simpl; trivial.
+
          + (*replace (get_numrec r + entry_numrec e - 1) with (get_numrec r) by lia.*)
-           clear. cancel. apply sepcon_derives. 2: admit. (*Tsh versus Ews -- fix specs*)
+           clear. cancel.
            subst currnode. Exists currnode_end. cancel. 
            fold btnode_rep. fold entry_rep. cancel.
       } {                       (* entryidx > numKeys isn't possible *)
@@ -384,24 +420,69 @@ Proof.
             + right. subst currnode r; apply H.
             + unfold correct_depth; subst r. lia. }
           forward.
-          { entailer. destruct e; [ unfold tentry in * | simpl in Hleaf; contradiction].
-            simpl. simpl in *. unfold tentry in H13.
-            rewrite value_fits_eq in H13; simpl in H13.
-            rewrite 2 value_fits_eq in H13; simpl in H13.
-            rewrite value_fits_eq in H13; simpl in H13.
-            assert (TC: tc_val (Tpointer tvoid noattr) v0) by admit. (*need tcval, not tcval'!!*)
-            apply prop_right. clear - TC. destruct v0; simpl in *; trivial. }
+          { entailer!. clear - H13 ENotVundef Hleaf.
+            destruct e; [ unfold tentry in * | simpl in Hleaf; contradiction].
+            simpl. simpl in *.
+            assert (TC: tc_val (Tpointer tvoid noattr) v0).
+            { rewrite value_fits_eq in H13; simpl in H13.
+              rewrite 2 value_fits_eq in H13; simpl in H13.
+              rewrite value_fits_eq in H13; simpl in H13.
+              apply H13; trivial. }
+            clear - TC. destruct v0; simpl in *; trivial. }
           simpl. rewrite SUBREP; clear SUBREP; Intros.
           rewrite unfold_btnode_rep at 1; Intros ent_end.
           forward.
           { entailer!. }
-          forward. simpl.
+          forward. (*simpl.
+          destruct e ; simpl in Hleaf; [ simpl in *| contradiction]. clear H4 H5 H6 EN EMPENTRY.
 Parameter listval:list val.
-          Exists listval.
+          Exists listval. rewrite putEntry_equation. simpl. rewrite H8.
+          remember (update_partial_cursor_rel c' (root, prel) (btnode val ptr0 (update_le (keyval val k v v0) le) true First Last x)) as updPC.
+          destruct updPC as [newc newr]. cancel.
+          specialize (update_partial_snd_r _ (root, prel) c' (btnode val ptr0 (update_le (keyval val k v v0) le) true First Last x)); simpl; intros HPrel.
+          destruct newr as [n prel0]; simpl; simpl in *.
+          rewrite <- HequpdPC in HPrel; simpl in HPrel; subst prel0.
+          assert (Lcc': Zlength newc = Zlength c').
+            { rewrite 2 Zlength_correct.
+              rewrite (update_partial_same_length _ c' (root, prel) (btnode val ptr0 (update_le (keyval val k v v0)le) true First Last x)).
+              rewrite <- HequpdPC; trivial. }
+          rewrite sepcon_comm. apply sepcon_derives.
+          { subst currnode; unfold cursor_rep; rewrite ! Zlength_cons. subst r. simpl. 
+            apply exp_derives. intros AE. apply exp_derives; intros IS. cancel.
+            rewrite Lcc'.
+            apply derives_refl'. f_equal. f_equal. f_equal. f_equal.
+            + f_equal. f_equal.
+              exploit (update_partial_cursor_result' root entryidx n prel c' newc (btnode val ptr0 (update_le (keyval val k v v0) le) true First Last x)).
+              trivial. intros XX; inv XX; trivial. (*maybe we're leaving an item of type node val on the shelf here*)
+            + apply update_partial_cursor_rel_getval in HequpdPC; rewrite HequpdPC; trivial. }
+          { cancel. subst r. Search btnode_rep. Locate LeafEntry_entry_numrec_one.
+            unfold complete_cursor, complete_cursor_correct_rel in H. simpl in H; destruct H.
+             Search subnode. (newc, (n, prel)) =
+           update_partial_cursor_rel c' (root, prel)
+             (btnode val ptr0 (update_le (keyval val k v v0) le) true First Last x):
+        (getval n = getval root /\ get_numrec (n, prel) = get_numrec (root, pefl) /\ get_depth (n, prel) = get_depth (root, prel))))) .
+
+
+Search btnode_rep. destruct newr as [xx prel0 ]destruct r0; simpl; simpl in Heqp. cancel.
+            subst r; simpl in *.
+            assert (n=root) by admit. subst n.
+            rewrite Vptrofs_repr_Vlong_repr; trivial. cancel.
+            admit. (*LHS of magic wand is too specific?*) }
+          
+            rewrite Lcc'. 
+            specialize update_partial_cursor_result'; intros XX.
+            apply derives_refl'. f_equal. f_equal. f_equal. f_equal.
+            + f_equal. f_equal.
+              specialize (XX root entryidx xx prel c' c (btnode val ptr0 (update_le e le) true First Last x)).
+              rewrite <- Heqp in XX. exploit XX; clear XX. trivial. intros XX; inv XX. rewrite H19; trivial.
+            + apply update_partial_cursor_rel_getval in Heqp; rewrite Heqp; trivial. }
+
+ (btnode val ptr0 (update_le e le) true First Last x)); rewrite <- Heqp; intros X; simpl in X; subst prel.
+          
+
           remember (putEntry val ((btnode val ptr0 le true First Last x, entryidx) :: c') (root, prel) e oldk listval nullval )
             as put; destruct put as [put1 put2].
-          assert (TSH_EWS: data_at Tsh tentry (entry_val_rep e) pe = data_at Ews tentry (entry_val_rep e) pe) by admit.
-          rewrite TSH_EWS; cancel.
+          cancel.
           rewrite putEntry_equation, H8 in Heqput.
           unfold update_currnode_cursor_rel in Heqput. simpl in Heqput.
           remember (update_partial_cursor_rel c' (root, prel) (btnode val ptr0 (update_le e le) true First Last x)) as p; destruct p; inv Heqput.
@@ -419,30 +500,13 @@ Parameter listval:list val.
             + f_equal. f_equal.
               specialize (XX root entryidx xx prel c' c (btnode val ptr0 (update_le e le) true First Last x)).
               rewrite <- Heqp in XX. exploit XX; clear XX. trivial. intros XX; inv XX. rewrite H19; trivial.
-            + f_equal. f_equal. simpl. destruct H as [HH1 HH2]; simpl in HH1, HH2. red in HH2. unfold complete_cursor_correct_rel in HH1. simpl in HH1. admit.
-(*
-Lemma update_partial_cursor_result'' root prel: forall c' c ptr le First Last x n b,
- (c, (n, prel)) =
-       update_partial_cursor_rel c' (root, prel) (btnode val ptr le b First Last x) ->
-(map fst c') = (map fst c).
-Proof. induction c'; simpl; intros. inv H. trivial.
-destruct a as [oldn i]. remember ( update_partial_cursor_rel c' (root, prel)
-         (update_node_nth_child i oldn (btnode val ptr le b First Last x))) as p. destruct p.
-inv H; simpl.
-remember (update_node_nth_child i oldn (btnode val ptr le b First Last x)). destruct n0.
-apply IHc' in Heqp. rewrite Heqp. f_equal.
-clear - Heqn0. rewrite Heqn0; clear Heqn0.
-unfold  update_node_nth_child. destruct oldn. destruct (zeq i (-1)); simpl.
-specialize (IHc' c0 n prel).  _ _ _ _ _ _ _ _ _ Heqp). 
-unfold update_node_nth_child in *. destruct n0; simpl in *.
-destruct (zeq z (-1)); simpl in *. destruct entryzero. admit.
-Print update_partial_cursor_rel .
-Print update_node_nth_child. Print update_le_nth_child.*) }
+            + apply update_partial_cursor_rel_getval in Heqp; rewrite Heqp; trivial. }
+
           { unfold relation_rep. destruct r0; simpl; simpl in Heqp. cancel.
             subst r; simpl in *.
             assert (n=root) by admit. subst n.
             rewrite Vptrofs_repr_Vlong_repr; trivial. cancel.
-            admit. (*LHS of magic wand is too specific?*) }
+            admit. (*LHS of magic wand is too specific?*) }*) admit.
             
 
         (* we need have key_in_le precisely at entry_index *)
@@ -495,13 +559,6 @@ Lemma gotokey_complete: forall c r key,
     complete_cursor c r ->
     complete_cursor (goToKey c r key) r.
 Proof.
-intros.
-destruct H.
-split; auto. red in H.
-unfold goToKey; red.
-remember (AscendToParent c key) as d; destruct d; simpl.
-+ apply AscendToParent_nil in Heqd. subst c. simpl in H; contradiction.
-+ 
 Admitted.
 
 Lemma putentry_complete: forall c r e oldk newx d newc newr,
@@ -511,6 +568,7 @@ Lemma putentry_complete: forall c r e oldk newx d newc newr,
 Proof.
 Admitted.
 
+(*Lennart: here's a partial proof- perhaps this is not true...*)
 Lemma putentry_depth: forall c r e oldk newx d newc newr,
     complete_cursor c r ->
     correct_depth r ->
@@ -518,6 +576,22 @@ Lemma putentry_depth: forall c r e oldk newx d newc newr,
     correct_depth newr.
 Proof.
 Admitted.
+(*Lennart: here's a partial proof- perhaps this is not true...
+unfold correct_depth. induction c; simpl; intros.
++ rewrite putEntry_equation in H1. destruct r as [root prel].
+  inv H1. simpl. unfold get_depth in *. simpl in *.
+  rewrite (Z.max_l _ 0). 2: apply entry_depth_nonneg.
+  admit.
++ rewrite putEntry_equation in H1. destruct r as [root prel]. destruct a as [n z].
+  destruct n. 
+  - remember (key_in_le (entry_key e) le) as b; destruct b.
+    * destruct isLeaf.
+      ++ inv H1. remember (update_partial_cursor_rel c (root, prel)
+          (btnode val entryzero (update_le e le) true First Last x)). destruct p.
+         inv H3. unfold get_depth in *; destruct newr; simpl in *. Search update_partial_cursor_rel.
+         admit.
+      ++ 
+Admitted.*)
 
 Lemma putentry_wf: forall c r e oldk newx d newc newr,
     complete_cursor c r ->
@@ -541,6 +615,7 @@ Lemma putentry_numrec: forall c r e oldk newx d newc newr,
     putEntry val c r e oldk newx d = (newc, newr) ->
     get_numrec newr < Int.max_signed.
 Proof.
+unfold get_numrec. intros. 
 Admitted.
 
 Lemma complete_depth: forall c r,
@@ -569,10 +644,10 @@ Proof.
     forward_call(c,pc,r,key).   (* gotokey(cursor,key) *)
     { split3; auto. unfold correct_depth. lia. }
     (*forward_call((goToKey c r key),pc,r,(keyval val key record recordptr), v_newEntry, key, gv).*) (* putEntry(cursor,newEntry,key *)
-    forward_call((goToKey c r key),pc,r,(keyval val key record (Vptrofs record)), v_newEntry, key, gv). (* putEntry(cursor,newEntry,key *)
-(*    + instantiate (Frame := []). apply force_val_sem_cast_neutral_isptr in H5. apply Some_inj in H5. rewrite <- H5.
-      rewrite <- H5.
-      simpl.
+    forward_call((goToKey c r key),pc,r,(keyval val key record (Vptrofs record)), v_newEntry, key, gv, Tsh). (* putEntry(cursor,newEntry,key *)
+    (*+ instantiate (Frame := []). apply force_val_sem_cast_neutral_isptr in H5. apply Some_inj in H5. rewrite <- H5.
+      rewrite <- H5.x
+      simpl. 
       simpl. replace((get_numrec r + 1 - 1)) with (get_numrec r) by lia. cancel.      
 *)
     + split3; auto. left. apply gotokey_complete. auto. apply I.
@@ -580,7 +655,7 @@ Proof.
       split3; auto.
       assert(complete_cursor (goToKey c r key) r) by (apply gotokey_complete; auto).
       apply eq_sym.
-      apply complete_depth. auto. auto. split; auto. lia.
+      apply complete_depth. auto. auto. split3; auto. discriminate. split. lia. apply writable_readable_share; apply writable_share_top.
     + Intros newx.
       destruct(putEntry val (goToKey c r key) r) as [newc newr] eqn:HPUTENTRY.
       forward_call(newc,pc,newr). (* RL_MoveToNext(cursor) *)
